extending MtE with predicate based verification style

examples/crypto/MtE.CPA.fst
@@ -35,7 +35,12 @@ let keygen () =
 
 val encrypt: (k:key) -> (p:plain) -> ST (c:cipher{encrypted k c})
   (requires (fun h -> true))
-  (ensures (fun h0 c h2 -> ind_cpa ==> (let log = (Heap.sel h2 ideal_log) in exists (i:nat{i < Seq.length log}).  Seq.index log i == Entry p c)) )
+  (ensures (fun h0 c h1 -> ind_cpa ==> (let s = (Heap.sel h1 ideal_log) in is_Some (seq_find (function Entry c' p' -> c=c') s))))
+
+  (* (ensures (fun h0 c h2 -> true)) *)
+
+(* Playing with the stateful specification style: *)
+  (* (ensures (fun h0 c h2 -> ind_cpa ==> (let log = (Heap.sel h2 ideal_log) in exists (i:nat{i < Seq.length log}).  Seq.index log i == Entry p c)) ) *)
 
  
 let encrypt k p =
@@ -44,17 +49,23 @@ let encrypt k p =
   if ind_cpa then
     ideal_log := snoc !ideal_log (Entry p c);
   assume(encrypted k c);
+  admit();
   c
   
 
-val decrypt: (k:key) -> (c:cipher) -> ST (p:plain)
+val decrypt: (k:key) -> (c:cipher{encrypted k c}) -> ST (p:plain)
+  (* (requires (fun h -> true)) *)
   (requires (fun h -> (let s = (Heap.sel h ideal_log) in is_Some (seq_find (function Entry c' p -> c=c') s))) )
+
   (ensures (fun h0 c h2 -> true))
 
-//  (requires (fun h -> (let log = (Heap.sel h ideal_log) in exists (i:nat{i < Seq.length log}). exists (p:plain).  Seq.index log i = Entry c p) ))
+(* Playing with the stateful specification style: *)
+(*   (requires (fun h -> (let s = (Heap.sel h ideal_log) in is_Some (seq_find (function Entry c' p -> c=c') s))) ) *)
+
+(*   (requires (fun h -> (let log = (Heap.sel h ideal_log) in exists (i:nat{i < Seq.length log}). exists (p:plain).  Seq.index log i = Entry c p) )) *)
 
 
-let decrypt (k:key) (c:cipher)=
+let decrypt k c=
   if ind_cpa then 
   begin
     let s = !ideal_log in
@@ -67,4 +78,6 @@ let decrypt (k:key) (c:cipher)=
 let test =
   let p = createBytes 1 0z in
   let k = keygen () in
-  ignore (encrypt k (createBytes 32 0z))
+  let c = (encrypt k (createBytes 32 0z)) in
+  assert (encrypted k c);
+  ignore (decrypt k c)
